SimAsm/SimAsm_Rules.thy
@@ -1,24 +1,43 @@
 theory SimAsm_Rules
-  imports SimAsm_WP
+  imports SimAsm_WP  
 begin
 
 
-instantiation state_rec_ext :: (type,type,type) pstate
+instantiation varmap_rec_ext :: (type,type,type) pstate
 begin
 
-definition "push_state_rec_ext \<equiv> \<lambda>(l :: ('a, 'b, 'c) state_rec_scheme) (r :: ('a, 'b, 'c) state_rec_scheme). l"
+definition "push_state_rec_ext \<equiv> \<lambda>(l :: ('a, 'b, 'c) varmap_rec_scheme) (r :: ('a, 'b, 'c) varmap_rec_scheme). l"
 
 instance (* Need to move some things around at the abstract level to get this through *)
   apply standard
   sorry
 end
 
+context wp
+begin
+
+print_locale wp
+
+(* ??? *)
+interpretation expression
+  "varmap_st"
+  "\<lambda>s v x. s\<lparr> varmap_st := (varmap_st s)(v := x)\<rparr>"
+  more
+  "\<lambda>s f. s\<lparr> more := f s\<rparr>"
+  "{x | x y. x = y }"     (*  Ul labelling makes all states labelled types *)
+by unfold_locales auto
+
+print_locale expression
+
+interpretation rules
+  done
+
 
 abbreviation lifted_abv ("_,_ \<turnstile>\<^sub>s _ {_} _" [20,0,0,0,20] 20)
-  where "lifted_abv R G P c Q \<equiv> step\<^sub>t R,step G \<turnstile> P {lift\<^sub>c c} Q" 
+  where "lifted_abv R G P c Q \<equiv> (step\<^sub>t R),(step G) \<turnstile> P {(lift\<^sub>c c)} Q" 
 
 abbreviation validity_abv  ("\<Turnstile> _ SAT [_, _, _, _]" [60,0,0,0] 45) 
-  where "validity_abv c P R G Q \<equiv> validity (lift\<^sub>c c) P (step\<^sub>t R) (step G) Q"
+ where "validity_abv c P R G Q \<equiv> validity (lift\<^sub>c c) P (step\<^sub>t R) (step G) Q" 
 
 text \<open>An ordering property on contexts\<close>
 definition context_order 
@@ -38,9 +57,10 @@ text \<open>Basic Rule for operations with vc\<close>
 lemma basic_wp\<^sub>i_1:
   assumes "P \<subseteq> stabilize R (c \<inter> wp\<^sub>i \<alpha> (wp\<^sub>a f Q))" "wellformed R G" "stable\<^sub>t R Q" 
   assumes "c \<subseteq> guar (wp\<^sub>i \<alpha> o wp\<^sub>a f) (step G)"
-  shows "step\<^sub>t R,step G \<turnstile> P {Basic (\<lfloor>c, \<alpha>, f\<rfloor>)} Q"
+  shows "(step\<^sub>t R),(step G) \<turnstile> P {Basic (liftg c \<alpha> f)} Q"
 proof -
-  have "step\<^sub>t R,step G \<turnstile>\<^sub>A stabilize R (c \<inter> wp\<^sub>i \<alpha> (wp\<^sub>a f Q)) {\<lfloor>c, \<alpha>, f\<rfloor>} Q"
+    have "(step\<^sub>t R),(step G) \<turnstile>\<^sub>A (stabilize R (c \<inter> wp\<^sub>i \<alpha> (wp\<^sub>a f Q))) {(liftg c \<alpha> f)} Q"
+(*  have "step\<^sub>t R,step G \<turnstile>\<^sub>A stabilize R (c \<inter> wp\<^sub>i \<alpha> (wp\<^sub>a f Q)) {\<lfloor>c, \<alpha>, f\<rfloor>} Q" *)
     using assms apply (cases \<alpha>) 
                 by (auto simp: atomic_rule_def guar_def wp_def step_def 
                                          wp\<^sub>r_def liftg_def o_def  elim!: stabilizeE) 
@@ -51,9 +71,9 @@ text \<open>Basic Rule for operations without vc\<close>
 lemma basic_wp\<^sub>i_2:
   assumes "P \<subseteq> stabilize R (wp\<^sub>i \<alpha> Q)" "wellformed R G" "stable\<^sub>t R Q"
   assumes "\<forall>m. m \<in> guar (wp\<^sub>i \<alpha>) (step G)"
-  shows "step\<^sub>t R,step G \<turnstile> P {Basic (\<lfloor>\<alpha>\<rfloor>)} Q"
+  shows "step\<^sub>t R,step G \<turnstile> P {Basic (liftl \<alpha>)} Q"
 proof -
-  have "step\<^sub>t R,step G \<turnstile>\<^sub>A stabilize R (wp\<^sub>i \<alpha> Q) {\<lfloor>\<alpha>\<rfloor>} Q"
+  have "step\<^sub>t R,step G \<turnstile>\<^sub>A stabilize R (wp\<^sub>i \<alpha> Q) {(liftl \<alpha>)} Q"
     using assms by (cases \<alpha>) (auto simp: atomic_rule_def guar_def wp_def step_def 
                                          wp\<^sub>r_def o_def liftl_def elim!: stabilizeE)
   thus ?thesis using assms by (intro conseq[OF basic]) (auto simp:)
@@ -63,7 +83,7 @@ text \<open>A rule for cmp operations, used for If/While\<close>
 lemma cmp_sound [intro!]:
   assumes "wellformed R G" "stable\<^sub>t R Q"
   assumes "P \<subseteq> stabilize R (wp\<^sub>i (cmp b) Q)"
-  shows "step\<^sub>t R,step G \<turnstile> P {Basic (\<lfloor>cmp b\<rfloor>)} Q"
+  shows "step\<^sub>t R,step G \<turnstile> P {Basic ((liftl (cmp b)))} Q"
   using assms by (intro basic_wp\<^sub>i_2) (auto simp: step_def reflexive_def wp\<^sub>r_def)
 
 subsection \<open>State Ordering\<close>
@@ -92,9 +112,9 @@ subsection \<open>Rules\<close>
 text \<open>If Rule\<close>
 
 lemma if_wp:
-  "R,G \<turnstile>\<^sub>w P\<^sub>1 {c\<^sub>1} Q' \<Longrightarrow> R,G \<turnstile>\<^sub>w P\<^sub>2 {c\<^sub>2} Q' \<Longrightarrow> R,G \<turnstile>\<^sub>w Q' {c\<^sub>3} Q \<Longrightarrow> 
-            R,G \<turnstile>\<^sub>w stabilize R (wp\<^sub>s (If b c\<^sub>1 c\<^sub>2 c\<^sub>3) Q) \<inter> 
-                    stabilize R (wp\<^sub>i (cmp b) P\<^sub>1 \<inter> wp\<^sub>i (ncmp b) P\<^sub>2) {If b c\<^sub>1 c\<^sub>2 c\<^sub>3} Q"
+  "R,G \<turnstile>\<^sub>w P\<^sub>1 {c\<^sub>1} Q \<Longrightarrow> R,G \<turnstile>\<^sub>w P\<^sub>2 {c\<^sub>2} Q \<Longrightarrow> 
+            R,G \<turnstile>\<^sub>w stabilize R (wp\<^sub>s (If b c\<^sub>1 c\<^sub>2) Q) \<inter> 
+                    stabilize R (wp\<^sub>i (cmp b) P\<^sub>1 \<inter> wp\<^sub>i (ncmp b) P\<^sub>2) {If b c\<^sub>1 c\<^sub>2} Q"
   unfolding valid_def apply clarsimp 
   apply (intro conjI)
   prefer 2
@@ -122,22 +142,21 @@ text \<open>While Rule\<close>
 lemma while_wp:
   assumes "R,G \<turnstile>\<^sub>w P {c} stabilize R J" (is "R,G \<turnstile>\<^sub>w P {c} ?I")
   assumes "J \<subseteq>  (wp\<^sub>i (cmp b) P \<inter> wp\<^sub>i (ncmp b) Q)"
-  shows "R,G \<turnstile>\<^sub>w ?I {While b J c} Q"
+  shows "R,G \<turnstile>\<^sub>w ?I {While b Imix Ispec c} Q"
   unfolding valid_def lift\<^sub>c.simps
-  sorry
-(*
 proof (intro impI conjI rules.choice rules.seq)
-  assume "wellformed R G \<and> stable\<^sub>t R Q \<and> guar\<^sub>c (While b J c) (G)"
-  thus "step\<^sub>t R,step G \<turnstile> ?I {(Basic (\<lfloor>cmp b\<rfloor>) ;; lift\<^sub>c c)*} ?I"
+  assume "wellformed R G \<and> stable\<^sub>t R Q \<and> guar\<^sub>c (While b Imix Ispec c) (G)"
+  thus "step\<^sub>t R,step G \<turnstile> ?I {(Seqw (Basic (liftl (cmp b))) (lift\<^sub>c c))*} ?I"
     using assms 
     apply (intro rules.loop rules.seq, unfold valid_def)
     apply force
-    apply force
-    apply (auto simp:)
-      apply (rule stabilize_entail, auto)+ 
-  done
+     apply force
+    apply (rule cmp_sound)
+      apply blast
+     apply (auto simp:)
+    using stabilize_entail by blast
 qed (insert assms, auto, rule stabilize_entail)
-*)
+
 
 text \<open>Do While Rule\<close>
 lemma do_wp:
@@ -182,7 +201,7 @@ lemma false_wp:
   assumes "P = {}"
   shows "R,G \<turnstile>\<^sub>w P {c} Q"
   using assms unfolding valid_def
-  by (intro conjI impI com_guar rules.conseq[OF falseI, where ?G="step G"]) (auto)
+  by (intro conjI impI rules.conseq[OF falseI, where ?G="step G"]) (auto)
 
 
 text \<open>Rewrite Rule\<close>
@@ -229,7 +248,7 @@ qed
 subsection \<open>High-Level Theorem\<close>
 
 text \<open>Soundness lemma for WP reasoning\<close>
-theorem armv8_wp_sound:
+theorem simAsm_wp_sound:
   assumes wf: "transitive R" "reflexive R" "reflexive G" 
   assumes st: "stable\<^sub>t R Q" 
   assumes g: "guar\<^sub>c c G"
@@ -241,5 +260,7 @@ proof -
   hence "R,G \<turnstile>\<^sub>s P {c} Q" by (rule rules.conseq) (insert P, auto simp: )
   thus ?thesis by (intro sound thread) auto
 qed
+
+end (* of context wp *)
 
 end
