SimAsm/Var_map.thy
@@ -28,14 +28,14 @@ type_synonym ('var,'val) varmap = "'var \<Rightarrow> 'val"
 datatype ('r,'v) op =
     assign "'r" "('r,'v) exp"
   | cmp "('r,'v) bexp"
+  | leak "'r" "('r,'v) exp"
   | full_fence
   | nop
-  | leak "'r" "('r,'v) exp"
 
 locale expression = state st st_upd aux aux_upd 
   for st :: "'s \<Rightarrow> 'r \<Rightarrow> 'v" 
   and st_upd ("_'((2_/ :=\<^sub>u/ (2_))')" [900,0,0] 901) and aux and aux_upd ("_'((2aux:/ _)')" [900,0] 901)
-  and locals :: "'r set" 
+(*  and locals :: "'r set"    Do we need local variables? *)
     
 
 (* context expression *)
